\documentclass[12pt,oneside,a4paper]{article}

\usepackage[utf8]{inputenc} % Lærer LaTeX at forstå unicode - HUSK at filen skal
% være unicode (UTF-8), standard i Linux, ikke i
% Win.

\usepackage{amsfonts}
\usepackage{amsthm}        % Theorems
\usepackage{amsmath}

\newcommand{\bas}{\begin{eqnarray*}}
\newcommand{\eas}{\end{eqnarray*}}
\newcommand{\be}{\begin{equation}}
\newcommand{\ee}{\end{equation}}
\newcommand{\bea}{\begin{eqnarray}}
\newcommand{\eea}{\end{eqnarray}}

\title{Pell's Equation}
\date{August 2022}
\author{Michael Jørgensen}

\begin{document}

\maketitle

\section{A problem}

Consider the sequence $(x_n, y_n)$ for $n=1, 2, 3, \ldots$ of positive integers $x_n$ and $y_n$.
They are required to satisfy the following recurrence relation:
%
\begin{eqnarray*}
    x_{n+1} &=& 2 x_n^2 - 1 \\
    y_{n+1} &=& 2 x_n y_n.
\end{eqnarray*}
%
The initial values $x_0$ and $y_0$ are required to satisfy
%
\begin{eqnarray*}
    x_0 &\ge& 2 \\
    y_0 &\ge& 1.
\end{eqnarray*}
%
These limitations guarantee that each of $x_n$ and $y_n$ diverge to infinity.

The task is to determine the following limit:
%
\begin{equation*}
    \lim_{n \rightarrow \infty} \frac{x_n}{y_n},
\end{equation*}
%
expressed in terms of the initial values $x_0$ and $y_0$.

\section{Examples}

With the initial values $(x_0, y_0) = (2, 1)$ we get the following table
%
\begin{equation*}
\begin{array}{c r r l}
    n &   x_n &    y_n & x_n/y_n \\
    0 &     2 &      1 & 2.0000 \\
    1 &     7 &      4 & 1.7500 \\
    2 &    97 &     56 & 1.7321 \\
    3 & 18817 & 100864 & 1.7321
\end{array}
\end{equation*}
%
This limit seems to converge to $\sqrt{3}$.

With the initial values $(x_0, y_0) = (3, 2)$ we get the following table
%
\begin{equation*}
\begin{array}{c r r l}
    n &    x_n &    y_n & x_n/y_n \\
    0 &      3 &      2 & 1.5000 \\
    1 &     17 &     12 & 1.4167 \\
    2 &    577 &    408 & 1.4142 \\
    3 & 665857 & 470832 & 1.4142
\end{array}
\end{equation*}
%
This limit seems to converge to $\sqrt{2}$.

\section{Solution outline}
Define
\begin{equation*}
    z_n = \frac{x_n^2-1}{y_n^2}.
\end{equation*}
Then determine a recurrence relation for $z_n$, which turns out to be simply
$z_{n+1} = z_n$.
%
We therefore have $z_n = z_0$, i.e.
\begin{equation*}
    \left(\frac{x_n}{y_n}\right)^2 - \frac{1}{y_n^2} = \frac{x_0^2-1}{y_0^2}.
\end{equation*}
%
Taking now the limit $n\rightarrow\infty$ on both sides gives the final result:
\begin{equation*}
    \lim_{n\rightarrow\infty} \frac{x_n}{y_n} = \frac{\sqrt{x_0^2-1}}{y_0}.
\end{equation*}

\section{Pell's equation}
Let $x_1$, $y_1$, and $d$ be positive integers satisfying
\begin{equation*}
    x_1^2 - d y_1^2 = 1
\end{equation*}
Now define $x_n$ and $y_n$ through the relation
\begin{equation*}
    x_n + \sqrt{d} y_n = \left(x_1 + \sqrt{d} y_1\right)^n.
\end{equation*}
Then we have
\begin{itemize}
    \item $$ x_n^2 - d y_n^2 = 1 $$
    \item $$ 
        \left( \begin{array}{c}
            x_{n+1} \\
            y_{n+1}
        \end{array} \right)
        = \left( \begin{array}{c c}
            x_1 & d y_1 \\
            y_1 & x_1
        \end{array} \right)
        \left( \begin{array}{c}
            x_{n} \\
            y_{n}
        \end{array} \right) $$
    \item 
        \begin{eqnarray*}
            x_{2n} &=& 2x_n^2 - 1 \\
            y_{2n} &=& 2x_ny_n
        \end{eqnarray*}
    \item $$ \lim_{n\rightarrow\infty} \frac{x_n}{y_n} = \sqrt{d} $$
    \item 
        \begin{eqnarray*}
            x_n &=& \frac12 \left(\lambda_1^n + \lambda_2^n\right) \\
            y_n &=& \frac1{2\sqrt{d}} \left(\lambda_1^n - \lambda_2^n\right) \\
            \lambda_1 &=& x_1 + \sqrt{d} y_1 = x_1 + \sqrt{x_1^2-1} \\
            \lambda_2 &=& x_1 - \sqrt{d} y_1 = x_1 - \sqrt{x_1^2-1} \\
            \lambda_1 \lambda_2 &=& 1
        \end{eqnarray*}
    \item
        \begin{eqnarray*}
            x_{n+1} &=& 2x_1x_n - x_{n-1} \\
            y_{n+1} &=& 2x_1y_n - y_{n-1}
        \end{eqnarray*}
    \item
        \begin{eqnarray*}
            x_n &=& T_n(x_1) \\
            y_n &=& U_{n-1}(x_1) y_1
        \end{eqnarray*}
    \item $$ \frac{x_n}{y_n} - \sqrt{d} \approx \frac{1}{2x_ny_n} $$

\end{itemize}


\end{document}

